{
 "cells": [
  {
   "cell_type": "markdown",
   "metadata": {},
   "source": [
    "Consider the quantum system with Hamiltonian\n",
    "$$H=\\frac{p^2}{2}+V(x) \\qquad [x,p]=i $$\n",
    "Suppose there exists $f(x)$ such that\n",
    "$$H=\\frac{f(x)-ip}{\\sqrt{2}}\\frac{f(x)+ip}{\\sqrt{2}}+\\varepsilon_0$$\n",
    "Comparing the both expressions we get that\n",
    "$$f'(x)=f^2(x)-2(V-\\varepsilon_0)$$\n",
    "Suppose there exists $\\psi(x)\\in L_2(\\mathbb{R})$:\n",
    "$$\\frac{f(x)+ip}{\\sqrt{2}} \\psi(x)=0$$\n",
    "Then $\\varepsilon_0$ и $\\psi$- energy and wave function of the ground state.\n",
    "$$\\psi'=-f(x)\\psi$$\n",
    "$$\\psi=N\\exp\\left(-\\int_{x_0}^x f(s) ds\\right)$$\n",
    "Average kinetic energy:\n",
    "$$<K>=\\int_{\\mathbb{R}}\\psi \\frac{p^2}{2} \\psi dx=-\\frac12\\int_{\\mathbb{R}}\\psi \\psi'' dx=\\frac12\\int_{\\mathbb{R}}\\psi \\psi'' dx=\\int_{\\mathbb{R}}\\frac{f^2}{2}\\psi^2 dx$$\n",
    "Average potential energy:\n",
    "$$<V>=\\int_{\\mathbb{R}} V(x)\\psi^2(x) dx=\\int_{\\mathbb{R}}\\left(\\varepsilon_0-\\frac{f'-f^2}{2}\\right)\\psi^2(x) dx$$\n",
    "Integration by paths:\n",
    "$$\\int_{\\mathbb{R}} f'\\psi^2 dx=-2\\int_{\\mathbb{R}} f\\psi'\\psi dx=2\\int_{\\mathbb{R}} f^2\\psi^2 dx$$\n",
    "$$<V>=\\varepsilon_0-\\int_{\\mathbb{R}} \\frac{f^2}{2} \\psi^2 dx$$\n",
    "$$<K>=<\\frac{f^2}{2}> \\qquad <V>=\\varepsilon_0-<\\frac{f^2}{2}>$$\n",
    "\n",
    "The simpliest example-harmonic oscillator\n",
    "\n",
    "$$\\tilde H=\\frac{P^2}{2m}+\\frac{m\\omega^2 X^2}{2} \\qquad [X,P]=i\\hbar$$\n",
    "We introduce dimensionless variables:\n",
    "    $$\\tilde H=E H \\quad X=Lx \\quad P=\\Pi p$$\n",
    "    $$E=\\hbar \\omega \\quad L=\\sqrt{\\frac{\\hbar}{m\\omega}} \\quad \\Pi=\\sqrt{\\hbar m \\omega}$$\n",
    "And we transform our problem to the previously considered type \n",
    "$$H=\\frac{p^2}{2}+\\frac{x^2}{2}$$\n",
    "$f(x)$ and $\\varepsilon_0$ for oscillator potential:\n",
    "$$f(x)=x \\qquad \\varepsilon_0=\\frac12$$\n",
    "wave function of the ground state:\n",
    "$$\\psi(x)=\\frac{1}{\\pi^{1/4}} e^{-x^2/2}$$\n",
    "Average values:\n",
    "$$<\\frac{f^2}{2}>=\\frac{1}{4} \\qquad <K>=<V>=\\frac{1}{4} $$\n",
    "We can express these values in terms of dimensional variables by the formulas:\n",
    "$$\\psi(x)\\to \\psi(X/L) \\frac{1}{\\sqrt{L}}$$\n",
    "$$<K>\\to E<K> \\quad <V> \\to E <V>$$\n",
    "$$<K>=<V>=\\frac14 \\hbar \\omega$$\n",
    "\n",
    "Morse potential:\n",
    "$$H=\\frac{P^2}{2m}+\\frac{g^2}{2}\\left[(e^{-qX}-1)^2-1\\right] \\qquad q>0$$\n",
    "By analogy with the oscillator, we introduce dimensionless variables using the following characteristic scales:\n",
    "$$E=g^2 \\qquad L=\\frac{\\hbar}{\\sqrt{m}g} \\qquad \\Pi=\\sqrt{m}g$$\n",
    "Hamiltonian takes the form:\n",
    "$$H=\\frac{p^2}{2}+\\frac12\\left[(e^{-\\alpha x}-1)^2-1\\right]$$\n",
    "where\n",
    "$$\\alpha=qL=\\frac{q\\hbar}{g\\sqrt{m}}>0$$\n",
    "is the dimensionless parametr.\n",
    "$$f(x)=-e^{-\\alpha x}+\\left(1-\\frac{\\alpha}{2}\\right)x \\qquad \\varepsilon_0=-\\frac{(2-\\alpha)^2}{8}$$\n",
    "$$\\psi=N\\exp\\left[-\\frac{1}{\\alpha}e^{-\\alpha x}-\\frac{2-\\alpha}{2}x\\right]$$\n",
    "Note, that bound states are exist only if $0<\\alpha<2$\n",
    "\n",
    "Average value of arbitrary function $\\varphi(x)$ is:\n",
    "$$<\\varphi(x)>=\\int_{\\mathbb{R}}\\varphi(x) \\psi^2(x) dx=\\int_{\\mathbb{R}}\\varphi(x) N^2\\exp\\left[-\\frac{2}{\\alpha}e^{-\\alpha x}-(2-\\alpha)x\\right]dx$$\n",
    "We substitute the variable:\n",
    "$$y=\\frac{2}{\\alpha}e^{-\\alpha x} \\qquad x=-\\frac{1}{\\alpha}\\ln\\left(\\frac{\\alpha}{2}y\\right)$$\n",
    "$$<\\varphi(x)>=\\frac{N^2}{2}\\left(\\frac{\\alpha}{2}\\right)^{\\frac{2}{\\alpha}-2}\\int_{\\mathbb{R}^{+}}\\varphi\\left(-\\frac{1}{\\alpha}\\ln\\left(\\frac{\\alpha}{2}y\\right)\\right)e^{-y}y^{\\frac{2-\\alpha}{\\alpha}-1} dy$$\n",
    "We calculate the normalizing factor, using the condition $<1>=1$:\n",
    "$$N^{-2}=\\frac{1}{2}\\left(\\frac{\\alpha}{2}\\right)^{\\frac{2}{\\alpha}-2}\\Gamma\\left(\\frac{2-\\alpha}{\\alpha}\\right)$$\n",
    "The main results: \n",
    "$$<\\varphi(x)>=\\int_{\\mathbb{R}^{+}}\\varphi\\left(-\\frac{1}{\\alpha}\\ln\\left(\\frac{\\alpha}{2}y\\right)\\right)\\frac{e^{-y}y^{\\frac{2-\\alpha}{\\alpha}-1}}{\\Gamma\\left(\\frac{2-\\alpha}{\\alpha}\\right)}dy$$\n",
    "$$<K>=<\\frac{f^2(x)}{2}>=\\frac{\\alpha}{4}\\left(1-\\frac{\\alpha}{2}\\right)$$\n",
    "$$<V>=\\varepsilon_0-<K>=\\frac{\\alpha}{4}-\\frac{1}{2}$$\n",
    "$$|\\psi|^2=\\frac{2^{1/\\alpha}(2-\\alpha)}{\\alpha^{3-2\\alpha}\\Gamma\\left(\\frac{2}{\\alpha}\\right)}\\exp\\left[-\\frac{2}{\\alpha}e^{-\\alpha x} -(2-\\alpha)x\\right]$$"
   ]
  },
  {
   "cell_type": "markdown",
   "metadata": {},
   "source": [
    "Consider the model of scalar field with (Euclidean) action:\n",
    "$$\\tilde A(\\varphi)=\\frac{1}{2}\\int\\left\\{\\dot\\varphi^2-q\\lambda e^{q\\varphi}+\\lambda^2e^{2q\\varphi}\\right\\}dt$$\n",
    "$$q<0 \\qquad \\lambda<0$$\n",
    "There are initional condition for the field $\\varphi$:\n",
    "$$\\varphi(0)=-\\infty$$\n",
    "Transform the action to the form:\n",
    "$$\\tilde A(\\varphi)=\\frac{1}{2}\\int\\left\\{\\dot\\varphi^2-\\lambda^2\\left[\\left(e^{q\\varphi}-\\frac{q}{2\\lambda}\\right)^2-\\left(\\frac{q}{2\\lambda}\\right)^2\\right]\\right\\}dt$$\n",
    "Transform the action by the following linear substitutions (the initial condition is invariant to these substitutions):\n",
    "\n",
    "$$\\varphi \\to \\theta_1 \\varphi+\\theta_2 \\qquad t \\to \\theta_3 t$$\n",
    "\n",
    "$$\\tilde A(\\varphi)=\\frac{1}{2}\\int\\left\\{\\frac{\\theta_1^2}{\\theta_3}\\dot\\varphi^2-\\lambda^2\\theta_3e^{2q\\theta_2}\\left[\\left(e^{q\\theta_1\\varphi}-\\frac{qe^{-q\\theta_2}}{2\\lambda}\\right)^2-\\left(\\frac{qe^{-q\\theta_2}}{2\\lambda}\\right)^2\\right]\\right\\}dt$$\n",
    "\n",
    "Сhoose the parameters equal to\n",
    "$$\\theta_1^2=\\theta_3 \\qquad e^{q\\theta_2}=\\frac{q}{2\\lambda}$$\n",
    "$$\\tilde A(\\varphi)=\\frac{1}{2}\\int\\left\\{ \\dot \\varphi^2+\\lambda^2\\left(\\frac{q}{2\\lambda}\\right)^2 \\theta_3\\left[(e^{q\\sqrt{\\theta_3} \\varphi}-1)^2-1\\right]\\right\\}dt$$\n",
    "$$\\theta_3=\\frac{4}{q^2} \\qquad \\sqrt{\\theta_3}=\\frac{2}{|q|} \\qquad q\\sqrt{\\theta_3}=-2$$\n",
    "The final form:\n",
    "$$\\tilde A(\\varphi)=\\frac{1}{2}\\int\\left\\{\\dot \\varphi^2+\\left[(e^{-2\\varphi}-1)^2-1\\right]\\right\\}dt$$\n",
    "So, this model is equivalent to previosly considered Morse potential with the parameter $\\alpha=2$ - there is no one bound state in this model!"
   ]
  },
  {
   "cell_type": "markdown",
   "metadata": {
    "collapsed": true
   },
   "source": [
    "$$\\Large{Path \\,\\, integral \\,\\, approximation}$$\n",
    "$$\\left<F\\right>=\\frac{1}{Z}Tr(e^{-\\beta H}F)=\\frac{\\sum_{n} e^{-\\beta E_n} F_n}{\\sum_{n} e^{-\\beta E_n}}=\\frac{F_0+\\sum_{n=1}e^{-\\beta (E_n-E_0)}F_n}{1+\\sum_{n=1}e^{-\\beta (E_n-E_0)}}\\to F_0 \\qquad \\beta \\to \\infty $$\n",
    "$$H|n>=E_n|n> \\qquad F_n=<n|F|n>$$\n",
    "$$\\rho_{\\beta}=\\frac{e^{-\\beta H}}{Tr\\left(e^{-\\beta H}\\right)}$$\n",
    "$$Tr(F\\rho_\\beta)=\\int dx dy <x|F|y><y|\\rho_\\beta|x>$$\n",
    "$$F=F(x) \\qquad <x|F|y>=F(x)\\delta(x-y) \\qquad <y|\\rho_\\beta|x>=\\frac{1}{Z}K(y,x,\\beta)$$\n",
    "$$\\left<F(x)\\right>=\\int \\frac{dx}{Z} F(x)K(x,x,\\beta)$$\n",
    "$$F=F(p) \\qquad <x|F(p)|y>=\\int dp <x|F(p)|p><p||y>=\\int dp F(p) <x||p> <p||y>=\\int \\frac{dp}{2\\pi} F(p)e^{ip(x-y)}=\\int \\frac{dp}{2\\pi} F(-i\\partial_x) e^{ip(x-y)}=F(-i\\partial_x)\\delta(x-y)$$\n",
    "$$<F(p)>=\\int dx dy F(-i\\partial_x)\\delta(x-y)K(y,x,\\beta)=\\int \\frac{dx}{Z} \\left[F(-i\\partial_y)K(y,x,\\beta)\\right]|_{y=x}$$\n",
    "\n",
    "$$\\rho_{\\beta_1}\\rho_{\\beta_2}=\\rho_{\\beta_1+\\beta_2}\\frac{Z(\\beta_1)Z(\\beta_2)}{Z(\\beta_1+\\beta_2)} \\qquad K(x,y,\\beta_1+\\beta_2)=\\int dz K(x,z,\\beta_1)K(z,y,\\beta_2)$$\n",
    "\n",
    "$$\\beta=Na \\qquad \\left<F(x)\\right>=\\int\\frac{dx_1...dx_N}{Z(\\beta)}K(x_1,x_N,a)...K(x_2,x_1,a) F(x_1)=\\frac{1}{N}\\sum_k\\int\\frac{dx_1...dx_N}{Z(\\beta)}K(x_1,x_N,a)...K(x_2,x_1,a) F(x_k)$$\n",
    "\n",
    "$$\\left<F(p)\\right>=\\int \\frac{dx_1}{Z} \\left[F(-i\\partial_y)K(y,x_1,\\beta)\\right]|_{y=x_1}=\\int \\frac{dx_1...dx_N}{Z} \\left[F(-i\\partial_y)K(y,x_2,a)\\right]|_{y=x_1}K(x_2,x_3,a)...K(x_N,x_1,a)=\\int \\frac{dx_1...dx_N}{Z}\\frac{\\left[F(-i\\partial_y)K(y,x_2,a)\\right]|_{y=x_1}}{K(x_1,x_2,a)}K(x_1,x_2,a)K(x_2,x_3,a)...K(x_N,x_1,a)=\\\\= \\frac{1}{N}\\sum_i\\int \\frac{dx_1...dx_N}{Z}\\frac{\\left[F(-i\\partial_y)K(y,x_{i+1},a)\\right]|_{y=x_i}}{K(x_i,x_{i+1},a)}K(x_1,x_2,a)K(x_2,x_3,a)...K(x_N,x_1,a)=\\left<\\frac{\\left[F(-i\\partial_y)K(y,x_{i+1},a)\\right]|_{y=x_i}}{K(x_i,x_{i+1},a)}\\right>$$\n",
    "\n",
    "$$K(x_2,x_1,a)=<x_2|e^{-aH}|x_1>=<x_2|e^{-a(T(p)+V(x))}|x_1>=<x_2|e^{-aT(p)}e^{-aV(x)}|x_1>+O(a^2)=\\int dz <x_2|e^{-aT(p)}|z><z|e^{-aV(x)}|x_1>=\\\\ \\int dz <x_2|e^{-aT(p)}|z> e^{-aV(x_1)} \\delta(z-x_1)=<x_2|e^{-aT(p)}|x_1>e^{-aV(x_1)}$$\n",
    "$$<x_2|e^{-aT(p)}|x_1>=\\int \\frac{dp}{2\\pi}e^{-aT(p)+ip(x_1-x_2)}$$\n",
    "$$T(p)=\\frac{p^2}{2m} \\qquad <x_2|e^{-aT(p)}|x_1>=e^{-m\\frac{(x_2-x_1)^2}{2a}}$$\n",
    "$$K(x_2,x_1,a)=e^{-m\\frac{(x_2-x_1)^2}{2a}-aV(x_1)}+O(a^2)$$\n",
    "$$\\left<F(x)\\right>=\\int\\frac{dx_1...dx_N}{Z}e^{-\\sum_i m\\frac{(x_{i+1}-x_i)^2}{2a}+aV(x_i)}F(x_1)=\\frac{1}{N}\\sum_k \\int\\frac{dx_1...dx_N}{Z}e^{-\\sum_i m\\frac{(x_{i+1}-x_i)^2}{2a}+aV(x_i)}F(x_k)$$\n",
    "$$\\left<\\frac{p^2}{2m}\\right>=\\frac{1}{2ma}\\left<1-\\frac{(x_{i+1}-x_i)^2}{a}\\right>=\\frac{1}{2ma}\\left<1-\\frac{x^2_i-2x_ix_{i+1}+x^2_{i+1}}{a}\\right>$$\n",
    "$$G_s=<x_ix_{i+s}>$$\n",
    "$$\\left<\\frac{p^2}{2m}\\right>=\\frac{1}{2ma}\\left(1-2\\frac{G_0-G_1}{a}\\right)$$\n"
   ]
  },
  {
   "cell_type": "markdown",
   "metadata": {},
   "source": [
    "$$\\Large{Monte-carlo}$$\n",
    "$$...$$"
   ]
  },
  {
   "cell_type": "markdown",
   "metadata": {},
   "source": [
    "$$\\Large{Green \\, \\, function}$$\n",
    "$$\\hat H=-\\frac12 \\partial_x^2+V(x)$$\n",
    "$$\\partial_t \\psi=-H\\psi \\qquad \\psi(x,0)=\\varphi(x)$$\n",
    "$$\\psi(x,t)=\\hat U(t) \\varphi(x)$$\n",
    "$$(\\partial_t \\hat U(t))\\varphi=-\\hat H \\hat U \\varphi \\qquad \\partial_t \\hat U=-\\hat H \\hat U$$\n",
    "$$\\psi(x,t)=\\hat U(t)\\varphi(x)=\\hat U(t)\\int_{\\mathbb{R}}dy \\delta(x-y)\\varphi(y)=\\int_{\\mathbb{R}}dy K(x,y,t)\\varphi(y) \\qquad K(x,y,t)=\\hat U(t) \\delta(x-y)$$\n",
    "inhomogeneous equation:\n",
    "$$\\partial_t \\psi=-H\\psi + f(x,t)$$\n",
    "\"variation of constant\"\n",
    "$$\\psi(x,t)=\\hat U(t) \\Phi(x,t)$$\n",
    "$$-HU\\Phi+U\\partial_t\\Phi=-HU\\Phi+f$$\n",
    "$$\\Phi(x,t)=\\varphi(x)+\\int_0^t \\hat U(-s) f(x,s) ds$$\n",
    "$$\\psi(x,t)=\\hat U(t)\\varphi(x)+\\int_0^t ds \\hat U(t-s) f(x,s)=\\int_{\\mathbb{R}}dy K(x,y,t) \\varphi(y)+\\int_0^t ds \\int_{\\mathbb{R}} dy K(x,y,t-s) f(x,s)$$\n",
    "$$\\varphi(x)=0 \\qquad f(x,t)=\\delta(x-x_0)\\delta(t) \\qquad \\psi(x,t)=K(x,x_0,t)$$"
   ]
  },
  {
   "cell_type": "markdown",
   "metadata": {
    "collapsed": true
   },
   "source": [
    "$$\\Large{Ito \\, \\, process}$$\n",
    "$$dx=a(x,t)dt+b(x,t)\\delta W$$\n",
    "$$\\partial_t u+\\partial_x(au)-\\frac{1}{2}\\partial^2_x(b^2u)=0$$\n",
    "\n",
    "$$\\partial_t \\psi=\\frac{1}{2}\\partial_x^2 - V\\psi$$\n",
    "$$u(x,t)=\\varphi(x)v(x,t)$$\n",
    "$$\\partial_t v+\\frac{\\partial_x(a\\varphi v)}{\\varphi}-\\frac{1}{2}\\frac{\\partial^2_x(b^2 \\varphi v)}{\\varphi}=0$$\n",
    "$$\\partial_t v-\\frac12 b^2 \\partial_x^2 v+\\left(a-\\frac{\\partial_x(b\\varphi)}{\\varphi}\\right)\\partial_x v+\\left[\\frac{\\partial_x(a\\varphi)}{\\varphi}-\\frac{\\partial_x^2(b^2\\varphi)}{2\\varphi}\\right]v=0$$\n",
    "$$-\\frac12b^2=-\\frac12$$\n",
    "$$a-\\frac{\\partial_x(b\\varphi)}{\\varphi}=0$$\n",
    "$$\\frac{\\partial_x(a\\varphi)}{\\varphi}-\\frac{\\partial^2_x(b^2\\varphi)}{2\\varphi}=V-\\varepsilon_0$$\n",
    "$$b=1 \\qquad a=a(x)=\\frac{\\varphi'}{\\varphi} \\qquad a'+a^2=2(V-\\varepsilon_0)$$\n",
    "$$a=-f(x) \\qquad f'=f^2-2(V-\\varepsilon_0)$$\n",
    "$$v=e^{\\varepsilon_0 t}\\psi(x,t) \\qquad \\partial_t\\psi=\\frac12\\partial_x^2 \\psi -V \\psi$$\n",
    "$$f'=f^2-2(V-\\varepsilon_0)$$\n",
    "$$dx=-f(x)dt+\\delta W \\Longrightarrow P(x,t)$$\n",
    "$$\\psi(x,t)=Ne^{\\int_{x_0}^x f(s) ds}e^{-\\varepsilon_0t}P(x,t)$$\n",
    "\n",
    "$$\\large{oscillator}$$\n",
    "$$V(x)=\\frac{x^2}{2} \\qquad f(x)=x \\qquad \\varepsilon_0=\\frac12 $$\n",
    "$$dx=-xdt+\\delta W$$\n",
    "-Ornstein Ulenbeck process\n",
    "\n",
    "method \"variation of constant\"\n",
    "$$x=y(t)e^{-t} \\qquad y=xe^t$$\n",
    "Ito's lemma:\n",
    "$$dy=\\left(\\frac{\\partial y}{\\partial t}+a\\frac{\\partial y}{\\partial x}+\\frac{b^2}{2}\\frac{\\partial^2 y}{\\partial x^2}\\right)dt+b\\frac{\\partial y}{\\partial x}\\delta W$$\n",
    "in our special case:\n",
    "$$dy=e^t \\delta W$$\n",
    "$$y(t)=x(0)+\\varepsilon\\sqrt{\\int_0^te^{2s}ds} \\qquad \\varepsilon\\sim\\mathbb{N}(0,1)$$\n",
    "$$x(t)=e^{-t}x(0)+\\varepsilon\\sqrt{\\frac12\\left(1-e^{-2t}\\right)} \\qquad x(t) \\sim \\mathbb{N}\\left(x_0 e^{-t},\\sqrt{\\frac12 \\left(1-e^{-2t}\\right)} \\right) \\qquad x_0\\equiv x(0)$$\n",
    "$$P(x,t)=\\frac{1}{\\sqrt{2\\pi}\\sqrt{\\frac{1-e^{-2t}}{2}}}\\exp\\left(\\frac{(x-x_0e^{-t})^2}{1-e^{-2t}}\\right)$$\n",
    "$$\\psi(x,t)=Ne^{-\\frac{x^2}{2}}e^{-t/2}\\frac{1}{\\sqrt{\\pi(1-e^{-2t})}}\\exp\\left(\\frac{(x-x_0e^{-t})^2}{1-e^{-2t}}\\right)=$$\n",
    "$$=\\frac{Ne^{-x_0^2/2}}{\\sqrt{2\\pi sht}}\\exp\\left(\\frac{x^2 cht + x_0^2 cht-2xx_0}{2sht}\\right)$$\n",
    "$$\\psi(x,t \\to 0) \\to Ne^{-x_0^2/2}\\delta(x-x_0)$$\n",
    "$$N=e^{x_0^2/2}$$\n",
    "$$\\psi(x,t)=\\frac{1}{\\sqrt{2\\pi sht}}\\exp\\left(\\frac{x^2 cht + x_0^2 cht-2xx_0}{2sht}\\right) \\qquad \\psi(x,0)=\\delta(x-x_0)$$\n",
    "$$K(x,x_0,t)=\\frac{1}{\\sqrt{2\\pi sht}}\\exp\\left(\\frac{x^2 cht + x_0^2 cht-2xx_0}{2sht}\\right)$$"
   ]
  },
  {
   "cell_type": "markdown",
   "metadata": {
    "collapsed": true
   },
   "source": [
    "$${\\LARGE Normalizing\\, \\,flow}$$\n",
    "$$x=f^{-1}(\\bar w,z)$$\n",
    "$$h(w,\\bar w,z)=f(w,f^{-1}(\\bar w,z)) \\qquad h(w,w,z)=z$$\n",
    "$$dh=H(w,\\bar w,z)dz \\qquad H(w,w,z)=I$$\n",
    "$$L[f]=\\frac{1}{N_{sample}}\\sum_{sample} \\ln\\tilde p_f(x)+S(x)$$\n",
    "$$\\tilde p_f(x)=r(f(w,x))\\left|det\\frac{\\partial f(w,x)}{\\partial x}\\right|$$\n",
    "rewrite in terms of functions of $z$:\n",
    "$$r(f(w,x))=r(f(w,f^{-1}(\\bar w,z)))=r(h(w,\\bar w,z))$$\n",
    "$$dh=\\left. \\frac{\\partial f(w,x)}{\\partial x}\\right|_{x=f^{-1}(\\bar w,z)} \\times \\frac{\\partial f^{-1}(\\bar w,z)}{\\partial z}dz=Hdz$$\n",
    "$$\\left. \\frac{\\partial f(w,x)}{\\partial x}\\right|_{x=f^{-1}(\\bar w,z)}=H \\times \\left(\\frac{\\partial f^{-1}(\\bar w,z)}{\\partial z}\\right)^{-1} $$\n",
    "$$L[f]=\\frac{1}{N_{sample}}\\sum_{sample}\\ln r\\left(h(w,\\bar w,z)\\right)+\\ln\\left|detH(w,\\bar w, z)\\right|-\\ln \\left|\\det\\frac{\\partial f^{-1}(\\bar w,z)}{\\partial z}\\right|+S(f(\\bar w,z)) \\equiv L(w,\\bar w)$$\n",
    "$$L(w,w)=\\frac{1}{N_{sample}}\\sum_{sample} S(f^{-1}(w,z))-\\ln \\left|\\det\\frac{\\partial f^{-1}(w,z)}{\\partial z}\\right|+const$$\n",
    "$$w' \\to w - lr \\times \\left[\\nabla_w \\left.L(w,\\bar w)\\right]\\right|_{w=\\bar w} $$"
   ]
  },
  {
   "cell_type": "markdown",
   "metadata": {},
   "source": [
    "$$....................................$$\n",
    "$$S(x)=\\frac12\\left(Ax,x\\right)$$\n",
    "$$f^{-1}(w,z)=wz$$\n",
    "$$\\mathcal{L}(w) \\equiv L(w,w)-const=\\frac12<(Awz,wz)>-\\ln\\det w=\\frac12tr\\left(w^TAw\\right)-\\ln|\\det w|$$\n",
    "$$O\\left(N_{nod}\\right)-\\mbox{invariance:} \\qquad \\mathcal{L}(wO)=\\mathcal{L}(w)$$\n",
    "$$\\mathcal{L}(w+\\varepsilon h)=\\frac12 tr\\left(w^TAw\\right)+\\frac{\\varepsilon}{2} tr(h^TAw+w^TAh)-\\ln|\\det(w+\\varepsilon h)|+o(\\varepsilon)$$\n",
    "$$\\ln|\\det(w+\\varepsilon h)|=\\ln\\left(|\\det(w)||\\det(I+\\varepsilon w^{-1}h)|\\right)=\\ln|\\det w|+\\ln(1+\\varepsilon tr\\left(w^{-1}h\\right))+o(\\varepsilon)=\\ln|\\det w|+\\varepsilon tr(w^{-1}h)$$\n",
    "$$\\mathcal{L}(w+\\varepsilon h)=\\mathcal{L}(w)+\\varepsilon tr(w^TAh)-\\varepsilon tr(w^{-1}h)=\\mathcal{L}(w)+\\varepsilon tr\\left([w^TA-w^{-1}]h\\right)=\\mathcal{L}(w)+\\varepsilon tr\\left([w^TA-w^{-1}]h\\right)=\\mathcal{L}(w)+\\varepsilon tr\\left([Aw-(w^T)^{-1}]^Th\\right)$$\n",
    "$$\\nabla \\mathcal{L}=Aw-(w^T)^{-1}$$"
   ]
  },
  {
   "cell_type": "markdown",
   "metadata": {},
   "source": [
    "$................................................................................................................................$"
   ]
  },
  {
   "cell_type": "markdown",
   "metadata": {
    "collapsed": true
   },
   "source": [
    "$$p(x)=\\frac{e^{-S(x)}}{Z} \\qquad x \\in \\mathbb{R}^N$$\n",
    "$$S(x)=\\sum_{k=1}^{N} \\frac{(x_{k+1}-x_k)^2}{2a}+aV(x_k)=\\frac{1}{2a}\\sum_{k=1}^N \\left( x_{k+1}^2-2x_kx_{k+1}+x_k^2+2a^2V(x_k) \\right)=\\frac{1}{2a}\\sum_{k=1}^N \\left( 2x_{k}^2+2a^2V(x_k)-2x_kx_{k+1} \\right)$$\n",
    "$$V(x)=\\frac{x^2}{2} \\qquad S(x)=\\frac{1}{2a}\\sum_{k=1}^N \\left( (2+a^2)x_{k}^2-2x_kx_{k+1} \\right)=\\frac{1}{2}(Ax,x) $$\n",
    "$$A=\\frac{1}{a}\\left((2+a^2)I-T-T^T\\right)$$\n",
    "$T$-generator of $\\mathbb{Z}_N$ (in regular representation)\n",
    "$$T=\\left(\\begin{array}{cccc}\n",
    "0 && 1 && ... && 0\\\\\n",
    "0 && 0 && 1 ... && 0\\\\\n",
    "... && ...&& ...&& ...\\\\\n",
    "... && ... &&  0 && 1\\\\\n",
    "1 && ... && ... && 0\n",
    "\\end{array}\\right)$$\n",
    "\n",
    "$$T_{i,k}=\\delta_{i+1,k} \\qquad T^{T}=T^{-1} \\qquad T^N=I$$\n",
    "$T$ can be diagonalized (by Schur's lemma)\n",
    "$$Tv=\\lambda v \\qquad T^Nv=\\lambda^Nv=v \\qquad \\lambda^N=1 \\qquad \\lambda_k=\\varepsilon^k \\quad \\varepsilon=e^{\\frac{2\\pi i}{N}}$$\n",
    "$$v_k=\\frac{1}{\\sqrt{N}}\\left( \\begin{array}{c}\n",
    "\\varepsilon^{0 k} \\\\\n",
    "\\varepsilon^{1k} \\\\\n",
    "\\varepsilon^{2k} \\\\\n",
    "...\\\\\n",
    "\\varepsilon^{(N-1)k}\n",
    "\\end{array} \\right)$$\n",
    "$$(v_n,v_m)=\\frac{1}{N}\\sum_{s=0}^{N-1} \\varepsilon^{s(m-n)}=$$\n",
    "$$=\\frac{1}{N}\\frac{\\varepsilon^{N(m-n)}-1}{\\varepsilon^{m-n}-1}=0 \\qquad \\mbox{in case $m\\ne n$}$$\n",
    "$$=1 \\qquad \\mbox{in case $n=m$} $$\n",
    "$$(v_n,v_m)=\\delta_{nm}$$\n",
    "$$Av_k=\\frac{1}{a}\\left((2+a^2)Iv_k-Tv_k-T^{-1}v_k\\right)=\\frac{1}{a}\\left(2+a^2-\\varepsilon^k-\\varepsilon^{-k}\\right)v_k=\\frac{1}{a}\\left(a^2+2-2\\cos\\left(\\frac{2\\pi k}{N}\\right)\\right)v_k=\\frac{1}{a}\\left(a^2+4\\sin^2\\left(\\frac{\\pi k}{N}\\right)\\right)v_k\\equiv\\Lambda_k v_k$$\n",
    "A-Hermitian, so there is a basis constructed from real eigenvectors of A.\n",
    "\n",
    "Case 1: N is even\n",
    "there are 2 real eigenvectors $v_0=\\frac{1}{\\sqrt{N}}(1,1,...,1)^T$ $v_{N/2}=\\frac{1}{\\sqrt{N}}(1,-1,1,...,-1)^T$ and $\\frac{N-2}{2}$ pairs of complex-conjugate vectors $v_k=\\frac{u_k+iw_k}{\\sqrt{2}}$ $v_{N-k}=\\frac{u_k-iw_k}{\\sqrt{2}}$\n",
    "\n",
    "Case 2: N is odd\n",
    "there is 1 real eigenvector $v_0=\\frac{1}{\\sqrt{N}}(1,1,...,1)^T$ and $\\frac{N-1}{2}$ pairs of complex-conjugate vectors $v_k=\\frac{u_k+iw_k}{\\sqrt{2}}$ $v_{N-k}=\\frac{u_k-iw_k}{\\sqrt{2}}$\n",
    "\n",
    "$$1=(v_k,v_k)=\\frac12(u_k,u_k)+\\frac12(w_k,w_k)$$\n",
    "$$0=(u_k-iw_k,u_k+iw_k)=\\frac12(u_k,u_k)-\\frac12(w_k,w_k)+i(u_k,w_k)$$\n",
    "$$(u_k,w_k)=0 \\qquad (u_k,u_k)=(w_k,w_k)=1$$\n",
    "$$u_k=\\sqrt{\\frac{2}{N}}\\left( \\begin{array}{c}\n",
    "1 \\\\\n",
    "\\cos\\left(\\frac{2\\pi k}{N}\\right) \\\\\n",
    "\\cos\\left(\\frac{4\\pi k}{N}\\right)\\\\\n",
    "...\\\\\n",
    "\\cos\\left(\\frac{2(N-1)\\pi k}{N}\\right)\n",
    "\\end{array} \\right) \\qquad w_k=\\sqrt{\\frac{2}{N}}\\left( \\begin{array}{c}\n",
    "0 \\\\\n",
    "\\sin\\left(\\frac{2\\pi k}{N}\\right) \\\\\n",
    "\\sin\\left(\\frac{4\\pi k}{N}\\right)\\\\\n",
    "...\\\\\n",
    "\\sin\\left(\\frac{2(N-1)\\pi k}{N}\\right)\n",
    "\\end{array} \\right)$$\n",
    "N-even:\n",
    "$$O=||v_0,u_1,w_1,...,u_{N/2-1},w_{N/2-1},v_{N/2}||$$\n",
    "N-odd:\n",
    "$$O=||v_0,u_1,w_1,...,u_{N/2-1},w_{N/2-1}||$$\n",
    "$$O^TO=I \\qquad O^TAO=diag(\\Lambda_0,\\Lambda_1,\\Lambda_1,...)$$\n",
    "$$n=diag\\left(\\frac{1}{\\sqrt{\\Lambda_0}},\\frac{1}{\\sqrt{\\Lambda_1}},\\frac{1}{\\sqrt{\\Lambda_1}},...\\right)$$\n",
    "$$C=On \\qquad C^TAC=I \\qquad A^{-1}=CC^T$$\n",
    "$$x=Cz \\qquad S(Cz)=\\frac12(z,z)  \\qquad p_z(z)=p_x(Cz) |det C|=(2\\pi)^{-N/2}e^{-\\frac{1}{2}(z,z)}$$\n",
    "\n",
    "consider random variable:\n",
    "$$\\eta_B=(Bz,z) \\qquad z\\sim\\mathcal{N}^N(0,1) \\qquad B^T=B$$\n",
    "$$M\\eta=B_{ik}\\delta_{ik}=trB$$\n",
    "$$M\\eta^2=B_{ik}B_{lm}M(z_iz_kz_lz_m)=B_{ik}B_{lm}(\\delta_{ik}\\delta_{lm}+\\delta_{il}\\delta_{km}+\\delta_{im}\\delta_{kl})=B_{ii}B_{ll}+B_{ik}B_{ik}+B_{ik}B_{ki}=(trB)^2+2trB^2$$\n",
    "$$D\\eta=2trB^2$$\n",
    "$$g_s=\\frac{1}{N}\\sum_{i=1}^Nx_{i}x_{i+s}=\\frac{1}{N}(T^sx,x)=\\frac{1}{N}(C^TT^sCz,z)=\\frac{1}{N}(C^{-1}A^{-1}T^sCz,z)$$\n",
    "$$G_s=Mg_s=\\frac{1}{N}tr(A^{-1}T^s)=\\frac{1}{N}tr(C^TT^sC)$$\n",
    "$$Dg_s=\\frac{2}{N^2}tr\\left((A^{-1}T^s)^2\\right)=\\frac{2}{N^2}tr\\left((C^TT^sC)^2\\right)$$\n",
    "$$G_0=\\sum_{k=0}^{N-1}\\frac{1}{N\\Lambda_k}=\\sum_{k=0}^{N-1}\\frac{1}{\\beta+\\frac{4N^2}{\\beta}sin^2\\left(\\frac{\\pi k}{N}\\right)}$$\n",
    "$$DG_0=2\\sum_{k=0}^{N-1} \\frac{1}{\\left(\\beta+\\frac{4N^2}{\\beta}\\sin^2\\left(\\frac{\\pi k}{N}\\right)\\right)^2}$$"
   ]
  },
  {
   "cell_type": "markdown",
   "metadata": {
    "collapsed": true
   },
   "source": [
    "$$............................................................................................$$\n",
    "The simpliest example-harmonic oscillator\n",
    "\n",
    "$$\\tilde H=\\frac{P^2}{2m}+\\frac{m\\omega^2 X^2}{2} \\qquad [X,P]=i\\hbar$$\n",
    "We introduce dimensionless variables:\n",
    "    $$\\tilde H=E H \\quad X=Lx \\quad P=\\Pi p$$\n",
    "    $$E=\\hbar \\omega \\quad L=\\sqrt{\\frac{\\hbar}{m\\omega}} \\quad \\Pi=\\sqrt{\\hbar m \\omega}$$\n",
    "And we transform our problem to the previously considered type \n",
    "$$H=\\frac{p^2}{2}+\\frac{x^2}{2}$$\n",
    "\n",
    "Relativistic oscillator\n",
    "$$\\tilde H=\\sqrt{P^2c^2+m^2c^4}+\\frac{m\\omega^2X^2}{2} \\qquad [X,P]=i\\hbar$$\n",
    "There are four dimension variables: $\\hbar, m, c, \\omega$\n",
    "\n",
    "Case1\n",
    "basic scales: $\\hbar, m, \\omega$\n",
    "$$\\Pi=\\sqrt{\\hbar m\\omega} \\qquad L=\\sqrt{\\frac{\\hbar}{m\\omega}} \\qquad E=\\hbar \\omega$$\n",
    "$$\\hbar \\omega H=\\sqrt{p^2\\hbar m \\omega c^2+m^2c^4}+\\frac{1}{2}\\frac{\\hbar}{ m \\omega}m\\omega^2 x^2 $$\n",
    "$$H=\\frac{1}{\\sigma}\\sqrt{p^2\\sigma+1}+\\frac{x^2}{2} \\qquad \\sigma=\\frac{\\hbar \\omega}{mc^2}$$\n",
    "non-relativistic:\n",
    "$$\\sigma<<1 \\qquad H=\\frac{p^2}{2}+\\frac{x^2}{2}+\\frac{1}{\\sigma}$$\n",
    "$$\\sigma>>1 \\qquad H=\\frac{|p|}{\\sqrt{\\sigma}}+\\frac{x^2}{2}$$\n",
    "\n",
    "Case2:\n",
    "basic scales: $\\hbar, \\omega, c$\n",
    "$$L=\\frac{c}{\\omega} \\qquad \\Pi=\\frac{\\hbar\\omega}{c} \\qquad E=\\hbar \\omega$$\n",
    "$$\\hbar \\omega H=\\sqrt{p^2c^2\\hbar^2\\omega^2/c^2+m^2c^4}+\\frac{m\\omega^2x^2}{2}\\frac{c^2}{\\omega^2}$$\n",
    "$$H=\\frac{1}{\\sigma}\\sqrt{p^2\\sigma^2+1}+\\frac{x^2}{2\\sigma} \\qquad \\sigma=\\frac{\\hbar \\omega}{mc^2}$$\n",
    "non-relativistic:\n",
    "$$\\sigma<<1 \\qquad H=\\frac{p^2\\sigma}{2}+\\frac{x^2}{2\\sigma}$$\n",
    "relativistic:\n",
    "$$\\sigma>>1 \\qquad H=|p|+\\frac{x^2}{2\\sigma}$$\n",
    "\n",
    "Case3: \n",
    "basic scales: $m,c,\\hbar$\n",
    "$$$$"
   ]
  },
  {
   "cell_type": "code",
   "execution_count": null,
   "metadata": {
    "collapsed": true
   },
   "outputs": [],
   "source": []
  }
 ],
 "metadata": {
  "kernelspec": {
   "display_name": "Python 3",
   "language": "python",
   "name": "python3"
  },
  "language_info": {
   "codemirror_mode": {
    "name": "ipython",
    "version": 3
   },
   "file_extension": ".py",
   "mimetype": "text/x-python",
   "name": "python",
   "nbconvert_exporter": "python",
   "pygments_lexer": "ipython3",
   "version": "3.6.2"
  }
 },
 "nbformat": 4,
 "nbformat_minor": 2
}
